formal/inference/heuristics/Instance_Of.thy
@@ -2,6 +2,8 @@ theory Instance_Of
   imports "../Inference"
 begin
 
-  
+definition just_do_it :: update_modifier where
+  "just_do_it t1ID t2ID s new old = (if Updates (get_by_id new t1ID) = [] then Some (replaceAll new (get_by_id new t1ID) (get_by_id new t2ID)) else
+                                     if Updates (get_by_id new t2ID) = [] then Some (replaceAll new (get_by_id new t2ID) (get_by_id new t1ID)) else None)"
 
 end
