formal/inference/Inference.thy
@@ -165,6 +165,10 @@ inductive satisfies_trace :: "execution \<Rightarrow> transition_matrix \<Righta
 definition satisfies :: "execution set \<Rightarrow> transition_matrix \<Rightarrow> bool" where
   "satisfies T e = (\<forall>t \<in> T. satisfies_trace t e 0 <>)"
 
+definition directly_subsumes :: "iEFSM \<Rightarrow> iEFSM \<Rightarrow> nat \<Rightarrow> transition \<Rightarrow> transition \<Rightarrow> bool" where
+  "directly_subsumes e1 e2 s t1 t2 \<equiv> (\<forall>p. accepts_trace (tm e1) p \<and> gets_us_to s (tm e1) 0 <>  p \<longrightarrow> subsumes t1 (anterior_context (tm e2) p) t2) \<and>
+                                     (\<exists>c. subsumes t1 c t2)"
+
 (* merge_transitions - Try dest merge transitions t\<^sub>1 and t\<^sub>2 dest help resolve nondeterminism in
                        newEFSM. If either subsumes the other directly then the subsumed transition
                        can simply be replaced with the subsuming one, else we try dest apply the
@@ -178,9 +182,9 @@ definition satisfies :: "execution set \<Rightarrow> transition_matrix \<Rightar
 (* @param modifier  - an update modifier function which tries dest generalise transitions           *)
 definition merge_transitions :: "iEFSM \<Rightarrow> iEFSM \<Rightarrow> transition \<Rightarrow> nat \<Rightarrow> transition \<Rightarrow> nat \<Rightarrow> update_modifier \<Rightarrow> iEFSM option" where
   "merge_transitions oldEFSM destMerge t\<^sub>1 u\<^sub>1 t\<^sub>2 u\<^sub>2 modifier = (
-     if directly_subsumes (tm oldEFSM) (tm destMerge) (origin u\<^sub>1 oldEFSM) t\<^sub>2 t\<^sub>1 then
+     if directly_subsumes oldEFSM destMerge (origin u\<^sub>1 oldEFSM) t\<^sub>2 t\<^sub>1 then
        Some (replace_transition destMerge u\<^sub>1 (origin u\<^sub>1 destMerge) (dest u\<^sub>2 destMerge) t\<^sub>1 t\<^sub>2)
-     else if directly_subsumes (tm oldEFSM) (tm destMerge) (origin u\<^sub>2 oldEFSM) t\<^sub>1 t\<^sub>2 then
+     else if directly_subsumes oldEFSM destMerge (origin u\<^sub>2 oldEFSM) t\<^sub>1 t\<^sub>2 then
        Some (replace_transition destMerge u\<^sub>1 (origin u\<^sub>1 destMerge) (dest u\<^sub>1 destMerge) t\<^sub>2 t\<^sub>1)
      else
         modifier u\<^sub>1 u\<^sub>2 (origin u\<^sub>1 destMerge) destMerge oldEFSM
